ToMathlib.lean
@@ -1,3 +1,4 @@
 import ToMathlib.General
+import ToMathlib.ExtDHashMapOfFintype
 import ToMathlib.ListFilterMap
 import ToMathlib.ListMapMOption
